theories/typing.v
@@ -4,20 +4,6 @@ From mathcomp Require Import ssreflect ssrfun ssrnat ssrbool eqtype seq.
 From Wasm Require Import operations.
 From Coq Require Import NArith.
 
-(**
-There are three files related to typing:
-  -- typing.v (this file): gives inductive definition of typing;
-  -- type_checker.v: gives a fixpoint that determines whether something is of 
-     a given type. This is somewhat like the interpreter, except that we need
-     to prove that typing is unique. I think it is already done for this
-     inductive definition but not for the type_checker yet? But that will follow
-     from the following..
-  -- type_checker_reflects_typing.v: gives a lemma that says the two above agree
-     with each other.
-
-  After all of these, we will need to prove preservation + progress with respect
-    to definitions in opsem.v. This should be in a separate file.
-**)
 
 Set Implicit Arguments.
 Unset Strict Implicit.
@@ -29,208 +15,219 @@ Variable host_function : eqType.
 
 Let function_closure := function_closure host_function.
 Let store_record := store_record host_function.
-(*Let administrative_instruction := administrative_instruction host_function.
-Let lholed := lholed host_function.*)
 
 
-(* TODO: Documentation *)
+(** std-doc:
+Helper function to decide if there's a valid conversion operation.
 
-(* FIXME: To which function in the Wasm specification does this correspond to? *)
-
-(** Answer to above
-
-  I searched through the specification but couldn't find a direct link to this either.
-    After some thoughts I think the only possibility is that this
-    is related to section 2.4.1, where all possible Convert operations are defined.
-
-  From my understanding, Cvtop is just a proxy for all the conversion operations, which
-    are the following (given in 2.4.1):
-    - i32.wrap_i64
-    - i64.extend_i32_sx
-    - inn.trunc_fmm_sx
-    - f32.demote_f64
-    - f64.promote_f32
-    - fnn.convert_imm_sx
-    - inn.reinterpret_fnn
-    - fnn.reinterpret_inn
-
-    where sx means the numbers are signed.
-
-    I think the original author wrote this convert_helper function for:
-      given two types t1, t2 and the sign option sx, if the function returns true,
-      then there is one of the above eight conversion operations that is
-      of the corresponding type (in fact one of the first six -- see below). 
-
-    For example, consider when will convert_helper be true if sxo is not None. In that
-      case we must have:
-      - at least one of t1 or t2 is not float;
-      - at least one of t1 or t2 is not int -- or if they are both int, then t1
-          should have length at least equal to t2.
-
-    Considering the fact that there are only 4 choices for t1,t2 (i/f 32/64), there
-      are only the following possible combinations that will make this function true
-      (noting that we need to have t1 and t2 being different):
-      - t1 = fnn, t2 = imm;
-      - t1 = inn, t2 = fmm;
-      - t1 = i64, t2 = i32.
-    These three combinations correspond exactly to the three signed conversions 
-      among the eight listed above (to trunc/convert/extend respectively).
-
-    When sx is unsigned, the helper function gives the three other conversions
-      that are not reinterpret operations. This is where we've been doing
-      differently from the official convention, since the official spec considers
-      reinterpret to be part of the conversion operations under the same proxy
-      (see 2.4.1.1). In our approach, Cvtop is only the proxy for the first 6 
-      conversion operations; we deal with the reinterpret operations in a separate
-      case (this is the case in both opsem.v and the be_typing function below).
-    
-    I guess it's fine if we keep it consistent within our own work, but I don't think
-      I'm the best person to decide this.
-
-    This might also answer some of the FIXMEs below.
-   
+See cvtop under: https://www.w3.org/TR/wasm-core-2/syntax/instructions.html#numeric-instructions
 **)
 Definition convert_helper (sxo : option sx) t1 t2 : bool :=
   (sxo == None) ==
-  ((is_float_t t1 && is_float_t t2) || (is_int_t t1 && is_int_t t2 && (t_length t1 < t_length t2))).
+  ((is_float_t t1 && is_float_t t2) || (is_int_t t1 && is_int_t t2 && (tnum_length t1 < tnum_length t2))).
 
-Definition convert_cond t1 t2 (sxo : option sx) : bool :=
+Definition convert_cond (t1 t2: number_type) (sxo : option sx) : bool :=
   (t1 != t2) && convert_helper sxo t1 t2.
 
 
-Definition upd_label C lab :=
+Definition upd_local_label_return C loc lab ret :=
   Build_t_context
-    (tc_types_t C)
-    (tc_func_t C)
-    (tc_global C)
+    (tc_type C)
+    (tc_func C)
     (tc_table C)
     (tc_memory C)
-    (tc_local C)
+    (tc_global C)
+    (tc_elem C)
+    (tc_data C)
+    loc
     lab
-    (tc_return C).
+    ret
+    (tc_ref C).
 
-(* FIXME: Change name *)
-(** This definition corresponds to the sentence
-    “The label C.labels[l] must be defined in the context.”
-    in the specification. **)
-Definition plop2 C i ts :=
-  List.nth_error (tc_label C) i == Some ts.
+Definition upd_local C loc :=
+  upd_local_label_return C loc (tc_label C) (tc_return C).
+
+Definition upd_label C lab :=
+  upd_local_label_return C (tc_local C) lab (tc_return C).
+
+Definition upd_return C ret :=
+  upd_local_label_return C (tc_local C) (tc_label C) ret.
+
 
 Inductive result_typing : result -> result_type -> Prop :=
   | result_typing_values : forall vs, result_typing (result_values vs) (map typeof vs)
   | result_typing_trap : forall ts, result_typing result_trap ts
   .
 
-Inductive unop_type_agree: value_type -> unop -> Prop :=
+Inductive unop_type_agree: number_type -> unop -> Prop :=
   | Unop_i32_agree: forall op, unop_type_agree T_i32 (Unop_i op)
   | Unop_i64_agree: forall op, unop_type_agree T_i64 (Unop_i op)
   | Unop_f32_agree: forall op, unop_type_agree T_f32 (Unop_f op)
   | Unop_f64_agree: forall op, unop_type_agree T_f64 (Unop_f op)
   .
    
-Inductive binop_type_agree: value_type -> binop -> Prop :=
+Inductive binop_type_agree: number_type -> binop -> Prop :=
   | Binop_i32_agree: forall op, binop_type_agree T_i32 (Binop_i op)
   | Binop_i64_agree: forall op, binop_type_agree T_i64 (Binop_i op)
   | Binop_f32_agree: forall op, binop_type_agree T_f32 (Binop_f op)
   | Binop_f64_agree: forall op, binop_type_agree T_f64 (Binop_f op)
   .
   
-Inductive relop_type_agree: value_type -> relop -> Prop :=
+Inductive relop_type_agree: number_type -> relop -> Prop :=
   | Relop_i32_agree: forall op, relop_type_agree T_i32 (Relop_i op)
   | Relop_i64_agree: forall op, relop_type_agree T_i64 (Relop_i op)
   | Relop_f32_agree: forall op, relop_type_agree T_f32 (Relop_f op)
   | Relop_f64_agree: forall op, relop_type_agree T_f64 (Relop_f op)
   .
+
+Definition is_numeric_type (t: value_type) : bool :=
+  match t with
+  | T_num _ => true
+  | T_vec _ => true
+  | _ => false
+  end.
+
   
-Inductive be_typing : t_context -> seq basic_instruction -> function_type -> Prop :=
-(** Corresponding to section 3.3 **)
+
+  
+(** std-doc:
+Instructions are classified by stack types that describe how instructions manipulate the operand stack.
+
+The types describe the required input stack with operand types that an instruction pops off and
+the provided output stack with result values of types that it pushes back. Stack types are akin 
+to function types, except that they allow individual operands to be classified as ⊥ (bottom), 
+indicating that the type is unconstrained. As an auxiliary notion, an operand type t1
+matches another operand type t2, if t1 is either ⊥ or equal to t2. This is extended to stack
+types in a point-wise manner.
+
+https://www.w3.org/TR/wasm-core-2/valid/instructions.html
+ **)
+Inductive be_typing : t_context -> seq basic_instruction -> function_type -> Type :=
 | bet_const : forall C v, be_typing C [::BI_const v] (Tf [::] [::typeof v])
 | bet_unop : forall C t op,
-    unop_type_agree t op -> be_typing C [::BI_unop t op] (Tf [::t] [::t])
+    unop_type_agree t op -> be_typing C [::BI_unop t op] (Tf [::T_num t] [::T_num t])
 | bet_binop : forall C t op,
-    binop_type_agree t op -> be_typing C [::BI_binop t op] (Tf [::t; t] [::t])
-| bet_testop : forall C t op, is_int_t t -> be_typing C [::BI_testop t op] (Tf [::t] [::T_i32])
+    binop_type_agree t op -> be_typing C [::BI_binop t op] (Tf [::T_num t; T_num t] [::T_num t])
+| bet_testop : forall C t op, is_int_t t -> be_typing C [::BI_testop t op] (Tf [::T_num t] [::T_num T_i32])
 | bet_relop: forall C t op,
-    relop_type_agree t op -> be_typing C [::BI_relop t op] (Tf [::t; t] [::T_i32])
+    relop_type_agree t op -> be_typing C [::BI_relop t op] (Tf [::T_num t; T_num t] [::T_num T_i32])
 | bet_convert : forall C t1 t2 sx, t1 <> t2 -> convert_helper sx t1 t2 ->
-  be_typing C [::BI_cvtop t1 CVO_convert t2 sx] (Tf [::t2] [::t1]) (* FIXME: Difference from the Isabelle formalisation: why merge the two rules here? *)
-| bet_reinterpret : forall C t1 t2, t1 <> t2 -> Nat.eqb (t_length t1) (t_length t2) ->
-  be_typing C [::BI_cvtop t1 CVO_reinterpret t2 None] (Tf [::t2] [::t1])
+  be_typing C [::BI_cvtop t1 CVO_convert t2 sx] (Tf [::T_num t2] [::T_num t1])
+| bet_reinterpret : forall C t1 t2, t1 <> t2 -> (tnum_length t1) = (tnum_length t2) ->
+  be_typing C [::BI_cvtop t1 CVO_reinterpret t2 None] (Tf [::T_num t2] [::T_num t1])
 | bet_unreachable : forall C ts ts',
   be_typing C [::BI_unreachable] (Tf ts ts')
 | bet_nop : forall C, be_typing C [::BI_nop] (Tf [::] [::])
 | bet_drop : forall C t, be_typing C [::BI_drop] (Tf [::t] [::])
-| bet_select : forall C t, be_typing C [::BI_select] (Tf [::t; t; T_i32] [::t])
-| bet_block : forall C tn tm es,
-  let tf := Tf tn tm in
-  be_typing (upd_label C (app [::tm] (tc_label C))) es (Tf tn tm) ->
-  be_typing C [::BI_block tf es] (Tf tn tm)
-| bet_loop : forall C tn tm es,
-  be_typing (upd_label C (app [::tn] (tc_label C))) es (Tf tn tm) ->
-  be_typing C [::BI_loop (Tf tn tm) es] (Tf tn tm)
-| bet_if_wasm : forall C tn tm es1 es2,
-  be_typing (upd_label C (app [::tm] (tc_label C))) es1 (Tf tn tm) ->
-  be_typing (upd_label C (app [::tm] (tc_label C))) es2 (Tf tn tm) ->
-  be_typing C [::BI_if (Tf tn tm) es1 es2] (Tf (app tn [::T_i32]) tm)
+| bet_select_Some : forall C t, be_typing C [::BI_select (Some [::t])] (Tf [:: t; t; T_num T_i32] [::t])
+| bet_select_None : forall C t, is_numeric_type t -> be_typing C [::BI_select None] (Tf [:: t; t; T_num T_i32] [::t])
+| bet_block : forall C tb tn tm es,
+  expand_t C tb = Some (Tf tn tm) ->
+  be_typing (upd_label C ([::tm] ++ (tc_label C))) es (Tf tn tm) ->
+  be_typing C [::BI_block tb es] (Tf tn tm)
+| bet_loop : forall C tb tn tm es,
+  expand_t C tb = Some (Tf tn tm) ->
+  be_typing (upd_label C ([::tn] ++ (tc_label C))) es (Tf tn tm) ->
+  be_typing C [::BI_loop tb es] (Tf tn tm)
+| bet_if_wasm : forall C tb tn tm es1 es2,
+  expand_t C tb = Some (Tf tn tm) ->
+  be_typing (upd_label C ([::tm] ++ (tc_label C))) es1 (Tf tn tm) ->
+  be_typing (upd_label C ([::tm] ++ (tc_label C))) es2 (Tf tn tm) ->
+  be_typing C [::BI_if tb es1 es2] (Tf (tn ++ [::T_num T_i32]) tm)
 | bet_br : forall C i t1s ts t2s,
-  i < length (tc_label C) ->
-  plop2 C i ts ->
-  be_typing C [::BI_br i] (Tf (app t1s ts) t2s)
+  List.nth_error C.(tc_label) (N.to_nat i) = Some ts ->
+  be_typing C [::BI_br i] (Tf (t1s ++ ts) t2s)
 | bet_br_if : forall C i ts,
-  i < length (tc_label C) ->
-  plop2 C i ts ->
-  be_typing C [::BI_br_if i] (Tf (app ts [::T_i32]) ts)
+  List.nth_error C.(tc_label) (N.to_nat i) = Some ts ->
+  be_typing C [::BI_br_if i] (Tf (ts ++ [::T_num T_i32]) ts)
 | bet_br_table : forall C i ins ts t1s t2s,
-  all (fun i => (i < length (tc_label C)) && (plop2 C i ts)) (app ins [::i])  ->
-  be_typing C [::BI_br_table ins i] (Tf (app t1s (app ts [::T_i32])) t2s)
+  List.Forall (fun i => (List.nth_error C.(tc_label) (N.to_nat i) = Some ts)) (ins ++ [::i])  ->
+  be_typing C [::BI_br_table ins i] (Tf (t1s ++ (ts ++ [::T_num T_i32])) t2s)
 | bet_return : forall C ts t1s t2s,
   tc_return C = Some ts ->
   be_typing C [::BI_return] (Tf (app t1s ts) t2s)
 | bet_call : forall C i tf,
-  i < length (tc_func_t C) ->
-  List.nth_error (tc_func_t C) i = Some tf ->
+  List.nth_error (tc_func C) (N.to_nat i) = Some tf ->
   be_typing C [::BI_call i] tf
-| bet_call_indirect : forall C i t1s t2s,
-  i < length (tc_types_t C) ->
-  List.nth_error (tc_types_t C) i = Some (Tf t1s t2s) ->
-  tc_table C <> nil -> (* TODO: this is redundant with the length check *)
-  be_typing C [::BI_call_indirect i] (Tf (app t1s [::T_i32]) t2s)
-| bet_get_local : forall C i t,
-  i < length (tc_local C) ->
-  List.nth_error (tc_local C) i = Some t ->
-  be_typing C [::BI_get_local i] (Tf [::] [::t])
-| bet_set_local : forall C i t,
-  i < length (tc_local C) ->
-  List.nth_error (tc_local C) i = Some t ->
-  be_typing C [::BI_set_local i] (Tf [::t] [::])
-| bet_tee_local : forall C i t,
-  i < length (tc_local C) ->
-  List.nth_error (tc_local C) i = Some t ->
-  be_typing C [::BI_tee_local i] (Tf [::t] [::t])
-| bet_get_global : forall C i t,
-  i < length (tc_global C) ->
-  option_map tg_t (List.nth_error (tc_global C) i) = Some t ->
-  be_typing C [::BI_get_global i] (Tf [::] [::t])
-| bet_set_global : forall C i g t,
-  i < length (tc_global C) ->
-  List.nth_error (tc_global C) i = Some g ->  
+| bet_call_indirect : forall C x y tabtype t1s t2s,
+  List.nth_error (tc_table C) (N.to_nat x) = Some tabtype ->
+  tabtype.(tt_elem_type) = T_funcref ->
+  List.nth_error (tc_type C) (N.to_nat y) = Some (Tf t1s t2s) ->
+  be_typing C [::BI_call_indirect x y] (Tf (t1s ++ [::T_num T_i32]) t2s)
+| bet_local_get : forall C x t,
+  List.nth_error (tc_local C) (N.to_nat x) = Some t ->
+  be_typing C [::BI_local_get x] (Tf [::] [::t])
+| bet_local_set : forall C x t,
+  List.nth_error (tc_local C) (N.to_nat x) = Some t ->
+  be_typing C [::BI_local_set x] (Tf [::t] [::])
+| bet_local_tee : forall C x t,
+  List.nth_error (tc_local C) (N.to_nat x) = Some t ->
+  be_typing C [::BI_local_tee x] (Tf [::t] [::t])
+| bet_global_get : forall C x t,
+  option_map tg_t (List.nth_error (tc_global C) (N.to_nat x)) = Some t ->
+  be_typing C [::BI_global_get x] (Tf [::] [::t])
+| bet_global_set : forall C x g t,
+  List.nth_error (tc_global C) (N.to_nat x) = Some g ->  
   tg_t g = t ->
   is_mut g ->
-  be_typing C [::BI_set_global i] (Tf [::t] [::])
+  be_typing C [::BI_global_set x] (Tf [::t] [::])
+| bet_table_get : forall C x tabtype t,
+  List.nth_error (tc_table C) (N.to_nat x) = Some tabtype ->
+  tabtype.(tt_elem_type) = t ->
+  be_typing C [::BI_table_get x] (Tf [::T_num T_i32] [::T_ref t])
+| bet_table_set : forall C x tabtype t,
+  List.nth_error (tc_table C) (N.to_nat x) = Some tabtype ->
+  tabtype.(tt_elem_type) = t ->
+  be_typing C [::BI_table_set x] (Tf [::T_num T_i32; T_ref t] [::])
+| bet_table_size : forall C x tabtype,
+  List.nth_error (tc_table C) (N.to_nat x) = Some tabtype ->
+  be_typing C [::BI_table_size x] (Tf [::] [::T_num T_i32])
+| bet_table_grow : forall C x tabtype t,
+  List.nth_error (tc_table C) (N.to_nat x) = Some tabtype ->
+  tabtype.(tt_elem_type) = t ->
+  be_typing C [::BI_table_grow x] (Tf [::T_ref t; T_num T_i32] [::T_num T_i32])
+| bet_table_fill : forall C x tabtype t,
+  List.nth_error (tc_table C) (N.to_nat x) = Some tabtype ->
+  tabtype.(tt_elem_type) = t ->
+  be_typing C [::BI_table_fill x] (Tf [::T_num T_i32; T_ref t; T_num T_i32] [::T_num T_i32])
+| bet_table_copy : forall C x y tabtype1 tabtype2 t,
+  List.nth_error (tc_table C) (N.to_nat x) = Some tabtype1 ->
+  tabtype1.(tt_elem_type) = t ->
+  List.nth_error (tc_table C) (N.to_nat y) = Some tabtype2 ->
+  tabtype2.(tt_elem_type) = t ->
+  be_typing C [::BI_table_copy x y] (Tf [::T_num T_i32; T_num T_i32; T_num T_i32] [::])
+| bet_table_init : forall C x y tabtype t,
+  List.nth_error (tc_table C) (N.to_nat x) = Some tabtype ->
+  tabtype.(tt_elem_type) = t ->
+  List.nth_error (tc_elem C) (N.to_nat y) = Some t ->
+  be_typing C [::BI_table_init x y] (Tf [::T_num T_i32; T_num T_i32; T_num T_i32] [::])
+| bet_elem_drop : forall C x t,
+  List.nth_error (tc_elem C) (N.to_nat x) = Some t ->
+  be_typing C [::BI_elem_drop x] (Tf [::] [::])
 | bet_load : forall C a off tp_sx t,
   tc_memory C <> nil ->
   load_store_t_bounds a (option_projl tp_sx) t ->
-  be_typing C [::BI_load t tp_sx a off] (Tf [::T_i32] [::t])
+  be_typing C [::BI_load t tp_sx a off] (Tf [::T_num T_i32] [::T_num t])
 | bet_store : forall C a off tp t,
   tc_memory C <> nil ->
   load_store_t_bounds a tp t ->
-  be_typing C [::BI_store t tp a off] (Tf [::T_i32; t] [::]) (* FIXME: Same here: two Isabelle rules have been merged here. *)
-| bet_current_memory : forall C,
+  be_typing C [::BI_store t tp a off] (Tf [::T_num T_i32; T_num t] [::])
+| bet_memory_size : forall C,
   tc_memory C <> nil ->
-  be_typing C [::BI_current_memory] (Tf [::] [::T_i32])
-| bet_grow_memory : forall C,
+  be_typing C [::BI_memory_size] (Tf [::] [::T_num T_i32])
+| bet_memory_grow : forall C,
   tc_memory C <> nil ->
-  be_typing C [::BI_grow_memory] (Tf [::T_i32] [::T_i32])
+  be_typing C [::BI_memory_grow] (Tf [::T_num T_i32] [::T_num T_i32])
+| bet_memory_fill : forall C,
+  tc_memory C <> nil ->
+  be_typing C [::BI_memory_fill] (Tf [::T_num T_i32; T_num T_i32; T_num T_i32] [::])
+| bet_memory_copy : forall C,
+  tc_memory C <> nil ->
+  be_typing C [::BI_memory_copy] (Tf [::T_num T_i32; T_num T_i32; T_num T_i32] [::])
+| bet_memory_init : forall C x,
+  tc_memory C <> nil ->
+  N.to_nat x < length (tc_data C) ->
+  be_typing C [::BI_memory_init x] (Tf [::T_num T_i32; T_num T_i32; T_num T_i32] [::])
 | bet_empty : forall C,
   be_typing C [::] (Tf [::] [::])
 | bet_composition : forall C es e t1s t2s t3s,
@@ -243,205 +240,67 @@ Inductive be_typing : t_context -> seq basic_instruction -> function_type -> Pro
 .
 
 
+(** std-doc:
+The following typing rules specify when a runtime store S is valid. A valid store must consist of
+ function, table, memory, global, and module instances that are themselves valid, relative to S.
 
-Definition upd_local C loc :=
-  Build_t_context
-    (tc_types_t C)
-    (tc_func_t C)
-    (tc_global C)
-    (tc_table C)
-    (tc_memory C)
-    loc
-    (tc_label C)
-    (tc_return C).
+To that end, each kind of instance is classified by a respective function, table, memory, or global
+ type. Module instances are classified by module contexts, which are regular contexts repurposed as
+ module types describing the index spaces defined by a module.
 
-Definition upd_return C ret :=
-  Build_t_context
-    (tc_types_t C)
-    (tc_func_t C)
-    (tc_global C)
-    (tc_table C)
-    (tc_memory C)
-    (tc_local C)
-    (tc_label C)
-    ret.
-
-Definition upd_local_return C loc ret :=
-  Build_t_context
-    (tc_types_t C)
-    (tc_func_t C)
-    (tc_global C)
-    (tc_table C)
-    (tc_memory C)
-    loc
-    (tc_label C)
-    ret.
-
-Definition upd_local_label_return C loc lab ret :=
-  Build_t_context
-    (tc_types_t C)
-    (tc_func_t C)
-    (tc_global C)
-    (tc_table C)
-    (tc_memory C)
-    loc
-    lab
-    ret.
-
-(**
- g_mut says whether the global is mutable; then it has another field g_val
-   specifying the value (with type).
- **)
-
-Definition global_agree (g : global) (tg : global_type) : bool :=
-  (tg_mut tg == g_mut g) && (tg_t tg == typeof (g_val g)).
-
-(**
- Determines if the nth element of gs is of global type tg. I felt that the first
-   condition isn't necessary since List.nth_error take care of it. This has been
-   the case for many other places as well. Maybe it's for eyeball-closeness?
+https://www.w3.org/TR/wasm-core-2/appendix/properties.html#store-validity
 **)
-Definition globals_agree (gs : seq global) (n : nat) (tg : global_type) : bool :=
-  (n < length gs) && (option_map (fun g => global_agree g tg) (List.nth_error gs n) == Some true).
+Section Store_validity.
 
-Definition mem_typing (m : memory) (m_t : memory_type) : bool :=
-  (N.leb m_t.(lim_min) (mem_size m)) &&
-  (m.(mem_max_opt) == m_t.(lim_max)) (* TODO: mismatch *).
-
-Definition memi_agree (ms : list memory) (n : nat) (mem_t : memory_type) : bool :=
-  (n < length ms) &&
-  match List.nth_error ms n with
-  | Some mem => mem_typing mem mem_t
-  | None => false
-  end.
-
-Definition functions_agree (fs : seq function_closure) (n : nat) (f : function_type) : bool :=
-  (n < length fs) && (option_map cl_type (List.nth_error fs n) == Some f).
-
-(*
-  This is the main point where the typing context in the typing system and the 
-    store in the operational semantics are connected. Writting my understanding down
-    for future reference since I'll definitely forget the meaning of some of them
-    at a point.
-
-  store_record and instance are from the operational semantics. 
-  Store_record contains 4 
-    components: 
-     - s_funcs, a sequence of function_closure;
-        function_closure is either a host, whose behaviour seems to be out of our
-          control; or a native function, which is of the form (Func_native i tf ts es).
-          here i is an instance, tf is the function type of this closure, ts is a 
-          sequence of value type (?) and es is a sequence of basic instruction.
-        Currently I don't see what this ts does (since basic instruction has EConst).
-          
-     - s_tab, a sequence of tabinst (tables);
-        Each table instance is basically a sequence of nat, with a limit on size.
-
-     - s_memory, a sequence of memory;
-        Similar to the above, though each memory is a sequence of byte instead of nat.
-
-     - s_glob, a sequence of global (global variables).
-        I think each is just one variable, could be either mutable/immutable, and could
-          be of the four wasm basic types (i/f 32/64).
-
-   Instance is for some reason very similar. It also has funcs, tab, memory and globs,
-     although they are all natural numbers or sequence of natural numbers (and for
-     some reason was named 'immediate'. There's an additional i_types which is a 
-     sequence of function_type (Tf t1s t2s).
-
-   t_context is the typing context used for the typing predicate. It contains
-     tc_types_t and tc_func_t which are both sequence of function_type; it also
-     contains tc_global, tc_table and tc_memory, although in t_context we only need
-     to know the types of these components. Tables and memories are typed by its 
-     size limit (TODO: need to update the definition in t_context), therefore 
-     tc_table and tc_memory are option of nat. tc_global is a sequence of global_type,
-     where each global_type is the type of one global (mutability + type).
-   The main difference is that t_context also contains tc_local, tc_label and tc_return.
-     I think this is what makes is really a 'context', as this implies that the current
-     sequence of instructions were taken from a larger overall picture. tc_local is 
-     a sequence of value_type (which turns out to be the 4 wasm basic types);
-     tc_label is a sequence of sequence of value_type (????), and tc_return is an
-     option on sequence of value_type.
-   I think we can try to deduce that by looking at the typing predicate above.
-   For tc_local we should probably look at instructions that manipulate local storage,
-     e.g. get/set/tee_local. We see in bet_get_local that get_local i would result in
-     function type [] -> [t] if the ith element of (tc_local C) is of type t. So
-     t_local stores the type of all local variables.
-   For tc_label, we should look at some control flow instructions that introduce new
-     labels. From the instruction 'Block': if we have an instruction 'Block tf es', and
-     tf = Tf tn tm, then the type of 'Block tf es' under context C is tn -> tm: but
-     this is at the condition that, in the modified typing context C', where we prepend
-     a 'tm' to tc_label of C, the instruction list es must be of type (Tf tn tm) as 
-     well. So it seems that tc_label keeps track of the resulting type of each label
-     in a stack?
-   It's probably better to look at where it is actually used. Check 'br': when we
-     see a 'Br i', we need that the length of tc_label C to be at least (i+1). This is
-     consistent with the above understanding since we need to have at least i+1 labels
-     present for the Br i instruction to be valid. We know Br i breaks from i labels and
-     continue execution at the continuation of the (i+1)th label. Then we find the 
-     ith entry of tc_label (0-indexed here), call it ts. The type of the break command
-     is then actually Tf (t1s ++ ts) t2s for arbitrary t1s and t2s!!?? This is actually
-     not a mistake (3.3.5.6). It is also weird that br_if doesn't have this 
-     polymorphism: it is always of type ts ++ [i32] -> ts. br_table is, however,
-     polymorphic again.
-  The reason for above is that  br_if is the only command that might not actually
-     break: if the top value is zero then we don't break. I think in Wasm, any if
-     command of this type must have the same type in both cases, therefore the case
-     that it actually breaks must also have the same type. The ts at the top of the
-     consumption is only there to demonstrate that this label indeed finishes with
-     a type of ts. The t2s can be whatever type that fits which makes the overall typing
-     consistent (I think): it is like in the separation logic course, where we give
-     br a reduction result of False (basically meaning that we never reach there, and
-     false deduces everything -- so if there are later commands we could be consistent).
-     The t1s part is to fit the accumulated type of the previous instructions, due to
-     definition of types of instruction sequences (3.3.6.2). In practice t1s will only
-     have one appropriate value that makes the overall typing work (and t2s also, if 
-     I'm correct). I think I'm indeed correct: later in the proof I should be able to
-     choose the correct t1s and t2s for the proof to work.
-
-   Ok now tc_return becomes obvious: it is the return type of the current function.
-     There is an analogy in the type of the return instruction which is very similar
-     to the 'Br i' instruction, being also polymorphic.
- *)
-
-(*
-  This basically says: an instance of a store_record has type C iff:
-  - i_types of instance is the same as tc_types_t of C;
-    It is unclear what this component actually is. What is this sequence of types?
-  - i_funcs of instance are indices of functions in the store. The type of the
-      each corresponding function in the store needs to have the same type as the
-      function in the typing_context;
-  - i_globs of instance are indices of globals in the store, and the same requirement
-      must be satisfied;
-  - i_tab specifies one index in the table sequence of the store. This table must be
-      of the same type as the table type in the typing context (typed by size limit);
-  - i_memory specifies one index in the memory sequence of the store, and the same
-      requirement must be satisfied;
-  - Then, the typing context has local vars, labels, and returns to be all empty.
- *)
+Definition funci_agree (fs : seq function_closure) (n : funcaddr) (f : function_type) : bool :=
+  option_map cl_type (List.nth_error fs n) == Some f.
 
 Definition tab_typing (t : tableinst) (tt : table_type) : bool :=
   (tt.(tt_limits).(lim_min) <= tab_size t) &&
-  (t.(table_max_opt) <= tt.(tt_limits).(lim_max)).
+  (t.(tableinst_type) == tt).
 
-Definition tabi_agree ts (n : nat) (tab_t : table_type) : bool :=
-  (n < List.length ts) &&
-  match List.nth_error ts n with
-  | None => false
-  | Some x => tab_typing x tab_t
-  end.
+Definition tabi_agree (ts: list tableinst) (n : tableaddr) (tab_t : table_type) : bool :=
+  option_map (fun tab => tab_typing tab tab_t) (List.nth_error ts n) == Some true.
 
+Definition mem_typing (m : meminst) (m_t : memory_type) : bool :=
+  (N.leb m_t.(lim_min) (mem_size m)) &&
+  (m.(meminst_type) == m_t).
+
+Definition memi_agree (ms : list meminst) (n : memaddr) (mem_t : memory_type) : bool :=
+  option_map (fun mem => mem_typing mem mem_t) (List.nth_error ms n) == Some true.
+
+Definition globali_agree (gs : list globalinst) (n : globaladdr) (tg : global_type) : bool :=
+  option_map g_type (List.nth_error gs n) == Some tg.
+
+(* TODO: figure out what's missing for elem/data/ref *)
+(** std-doc:
+https://www.w3.org/TR/wasm-core-2/appendix/properties.html#module-instances-xref-exec-runtime-syntax-moduleinst-mathit-moduleinst
+**)
 Definition inst_typing (s : store_record) (inst : instance) (C : t_context) : bool :=
-  let '{| inst_types := ts; inst_funcs := fs; inst_tab := tbs; inst_memory := ms; inst_globs := gs; |} := inst in
+  let '{| inst_types := ts; inst_funcs := fs; inst_tables := tbs; inst_mems := ms; inst_globals := gs;
+       inst_elems := es; inst_datas := ds; inst_exports := exps |} := inst in
   match C with
-  | {| tc_types_t := ts'; tc_func_t := tfs; tc_global := tgs; tc_table := tabs_t; tc_memory := mems_t; tc_local := nil; tc_label := nil; tc_return := None |} =>
+  | {| tc_type := ts'; tc_func := tfs; tc_table := tabs_t; tc_memory := mems_t; tc_global := tgs; tc_elem := nil; tc_data := nil; tc_local := nil; tc_label := nil; tc_return := None; tc_ref := nil; |} =>
     (ts == ts') &&
-    (all2 (functions_agree s.(s_funcs)) fs tfs) &&
-    (all2 (globals_agree s.(s_globals)) gs tgs) &&
+    (all2 (funci_agree s.(s_funcs)) fs tfs) &&
+    (all2 (globali_agree s.(s_globals)) gs tgs) &&
     (all2 (tabi_agree s.(s_tables)) tbs tabs_t) &&
     (all2 (memi_agree s.(s_mems)) ms mems_t)
   | _ => false
   end.
+
+
+Lemma inst_typing_expand (s: store_record) (inst: instance) (C: t_context) (tb: block_type) :
+  inst_typing s inst C ->
+  expand inst tb = expand_t C tb.
+Proof.
+  destruct tb, inst, C => //=.
+  destruct tc_elem, tc_data, tc_local, tc_label, tc_return, tc_ref => //.
+  move => Htype.
+  repeat (move/andP in Htype; destruct Htype as [Htype _]).
+  by move/eqP in Htype; subst.
+Qed.
+
 
 Inductive frame_typing: store_record -> frame -> t_context -> Prop :=
 | mk_frame_typing: forall s i tvs C f,
@@ -452,44 +311,17 @@ Inductive frame_typing: store_record -> frame -> t_context -> Prop :=
   .
 
 Lemma functions_agree_injective: forall s i t t',
-  functions_agree s i t ->
-  functions_agree s i t' ->
+  funci_agree s i t ->
+  funci_agree s i t' ->
   t = t'.
 Proof.
   move => s i t t' H1 H2.
-  unfold functions_agree in H1. unfold functions_agree in H2.
-  (*move/andP in H1. move/andP in H2.*)
-  move/andP: H1 => [_ H1].
-  move/andP: H2 => [_ H3].
-  move/eqP in H1. move/eqP in H3.
-  rewrite H3 in H1 => {H3}.
+  unfold funci_agree in *.
+  move/eqP in H1. move/eqP in H2.
+  rewrite H2 in H1 => {H2}.
   by move: H1 => [H1].
 Qed.
 
-(*
-Print Func_native.
-
-  Here we're typing a function closure. The second case where we have a host function
-    is obvious: it can be anything.
-  However, if it is a native function, then we should be able to deduce its type.
-    Suppose we have a store s. The function is based on an instance i, and claims to
-    have type tf = (T1s -> T2s). It also comes with a sequence of local variables of
-    type ts (think parameters). The body of the function is es.
-  Let C be a typing context for the instance i of the store s. Because of the local
-    variables, we append ts to the local part of the typing context C. Then we 
-    prepend a t1s in the local section and a t2s in the label section since that is the
-    outermost block (think reduction result of admin instruction [::Local ...]). The
-    result, which is t2s, is also updated into the typing context. Let this modified
-    typing context be C' (I'm not sure why these are necessary though).
-  Then, this native function Func_native i tf ts es indeed has its claimed type 
-    t1s -> t2s iff under this typing context C', its function body es has type
-    [::] -> t2s, i.e. consuming nothing (since there's nothing in the stack) and 
-    producing some results with type t2s. The type of the body es is fully determined
-    by be_typing.
-
-  I think the main use of this is for typing the Callcl (now renamed to Invoke)
-    instructions.
- *)
 Inductive cl_typing : store_record -> function_closure -> function_type -> Prop :=
   | cl_typing_native : forall i s C C' ts t1s t2s es tf,
     inst_typing s i C ->
@@ -501,10 +333,14 @@ Inductive cl_typing : store_record -> function_closure -> function_type -> Prop 
     cl_typing s (FC_func_host tf h) tf
   .
 
-(*
-  e_typing is the extension of typing to administrative instructions. See appendix 5 for
-    some of them.
-*)
+(** std-doc:
+Typing rules for administrative instructions are specified as follows. In addition to the context C, typing
+ of these instructions is defined under a given store S. To that end, all previous typing judgements are 
+generalized to include the store by implicitly adding S to all rules – S is never modified by the 
+pre-existing rules, but it is accessed in the extra rules for administrative instructions given below.
+
+https://www.w3.org/TR/wasm-core-2/appendix/properties.html#administrative-instructions
+**)
 
 Inductive e_typing : store_record -> t_context -> seq administrative_instruction -> function_type -> Prop :=
 | ety_a : forall s C bes tf,
@@ -518,11 +354,12 @@ Inductive e_typing : store_record -> t_context -> seq administrative_instruction
   e_typing s C es (Tf (ts ++ t1s) (ts ++ t2s))
 | ety_trap : forall s C tf,
   e_typing s C [::AI_trap] tf
-| ety_local : forall s C n f es ts,
-  s_typing s (Some ts) f es ts ->
-  length ts = n ->
-  e_typing s C [::AI_local n f es] (Tf [::] ts)
-| ety_invoke : forall s a C cl tf,
+| ety_ref_extern : forall s C a,
+  e_typing s C [::AI_ref_extern a] (Tf [::] [::T_ref T_externref])
+| ety_ref : forall s C a tf,
+  funci_agree s.(s_funcs) a tf ->
+  e_typing s C [::AI_ref a] (Tf [::] [::T_ref T_funcref])
+| ety_invoke : forall s (a: funcaddr) C cl tf,
   List.nth_error s.(s_funcs) a = Some cl ->
   cl_typing s cl tf ->
   e_typing s C [::AI_invoke a] tf
@@ -531,6 +368,10 @@ Inductive e_typing : store_record -> t_context -> seq administrative_instruction
   e_typing s (upd_label C ([::ts] ++ tc_label C)) es (Tf [::] t2s) ->
   length ts = n ->
   e_typing s C [::AI_label n e0s es] (Tf [::] t2s)
+| ety_local : forall s C n f es ts,
+  s_typing s (Some ts) f es ts ->
+  length ts = n ->
+  e_typing s C [::AI_local n f es] (Tf [::] ts)
 
 with s_typing : store_record -> option (seq value_type) -> frame -> seq administrative_instruction -> seq value_type -> Prop :=
 | mk_s_typing : forall s f es rs ts C C0,
@@ -557,40 +398,37 @@ Qed.
 Definition cl_type_check_single (s:store_record) (f:function_closure):=
   exists tf, cl_typing s f tf.
 
-Definition tabcl_agree (s : store_record) (tcl_index : option nat) : Prop :=
-  match tcl_index with
-  | None => True
-  | Some n => n < size s.(s_funcs)
-(*  let tcl := List.nth_error (s_funcs s) n in
-    match tcl with
-    | None => False
-    | Some cl => cl_type_check_single s cl
-    end*)
+Definition tabcl_agree (s : store_record) (tref: reference_type) (v : value_ref) : Prop :=
+  match v with
+  | VAL_ref_null tref' => tref = tref'
+  | VAL_ref_func a => (a < length s.(s_funcs)) /\ (tref = T_funcref)
+  | VAL_ref_extern _ => tref = T_externref
   end.
 
 Definition tabsize_agree (t: tableinst) : Prop :=
-  match table_max_opt t with
+  match t.(tableinst_type).(tt_limits).(lim_max) with
   | None => True
   | Some n => tab_size t <= n
   end.
 
 Definition tab_agree (s: store_record) (t: tableinst): Prop :=
-  List.Forall (tabcl_agree s) (t.(table_data)) /\
+  List.Forall (tabcl_agree s t.(tableinst_type).(tt_elem_type)) (t.(tableinst_elem)) /\
   tabsize_agree t.
 
-Definition mem_agree (m : memory) : Prop :=
-  match (mem_max_opt m) with
+Definition mem_agree (m : meminst) : Prop :=
+  match m.(meminst_type).(lim_max) with
   | None => True
-  | Some n => N.le (mem_size m) n
+  | Some n => mem_size m <= n
   end.
 
 Definition store_typing (s : store_record) : Prop :=
   match s with
-  | Build_store_record fs tclss mss gs =>
+  | Build_store_record fs tclss mss gs es ds =>
     List.Forall (cl_type_check_single s) fs /\
     List.Forall (tab_agree s) tclss /\
     List.Forall mem_agree mss
   end.
+
 
 Inductive config_typing : store_record -> frame -> seq administrative_instruction -> seq value_type -> Prop :=
 | mk_config_typing :
@@ -598,6 +436,8 @@ Inductive config_typing : store_record -> frame -> seq administrative_instructio
   store_typing s ->
   s_typing s None f es ts ->
   config_typing s f es ts.
+
+End Store_validity.
 
 
 End Host.
