theories/opsem.v
@@ -2,7 +2,7 @@
 (** The interpreter in the [interpreter] module is an executable version of this operational semantics. **)
 (* (C) J. Pichon, M. Bodin - see LICENSE.txt *)
 
-From Coq Require Import ZArith.BinInt.
+From Coq Require Import ZArith.BinInt NArith.BinNat.
 From mathcomp Require Import ssreflect ssrfun ssrnat ssrbool eqtype seq.
 Require Export operations host.
 
@@ -19,50 +19,49 @@ Let host := host host_function.
 Variable host_instance : host.
 
 Let store_record := store_record host_function.
-(*Let administrative_instruction := administrative_instruction host_function.*)
 Let host_state := host_state host_instance.
 
 Inductive reduce_simple : seq administrative_instruction -> seq administrative_instruction -> Prop :=
 
 (** unop **)
   | rs_unop : forall v op t,
-    reduce_simple [::AI_basic (BI_const v); AI_basic (BI_unop t op)] [::AI_basic (BI_const (@app_unop op v))]
+    reduce_simple [::$VA v; AI_basic (BI_unop t op)] [::$VA (@app_unop op v)]
                    
 (** binop **)
   | rs_binop_success : forall v1 v2 v op t,
     app_binop op v1 v2 = Some v ->
-    reduce_simple [::AI_basic (BI_const v1); AI_basic (BI_const v2); AI_basic (BI_binop t op)] [::AI_basic (BI_const v)]
+    reduce_simple [::$VA v1; $VA v2; AI_basic (BI_binop t op)] [::$VA v]
   | rs_binop_failure : forall v1 v2 op t,
     app_binop op v1 v2 = None ->
-    reduce_simple [::AI_basic (BI_const v1); AI_basic (BI_const v2); AI_basic (BI_binop t op)] [::AI_trap]
+    reduce_simple [::$VA v1; $VA v2; AI_basic (BI_binop t op)] [::AI_trap]
                   
   (** testops **)
   | rs_testop_i32 :
     forall c testop,
-    reduce_simple [::AI_basic (BI_const (VAL_int32 c)); AI_basic (BI_testop T_i32 testop)] [::AI_basic (BI_const (VAL_int32 (wasm_bool (@app_testop_i i32t testop c))))]
+    reduce_simple [::$VA (VAL_int32 c); AI_basic (BI_testop T_i32 testop)] [::$VA (VAL_int32 (wasm_bool (@app_testop_i i32t testop c)))]
   | rs_testop_i64 :
     forall c testop,
-    reduce_simple [::AI_basic (BI_const (VAL_int64 c)); AI_basic (BI_testop T_i64 testop)] [::AI_basic (BI_const (VAL_int32 (wasm_bool (@app_testop_i i64t testop c))))]
+    reduce_simple [::$VA (VAL_int64 c); AI_basic (BI_testop T_i64 testop)] [::$VA (VAL_int32 (wasm_bool (@app_testop_i i64t testop c)))]
 
   (** relops **)
   | rs_relop: forall v1 v2 t op,
-    reduce_simple [::AI_basic (BI_const v1); AI_basic (BI_const v2); AI_basic (BI_relop t op)] [::AI_basic (BI_const (VAL_int32 (wasm_bool (app_relop op v1 v2))))]
+    reduce_simple [::$VA v1; $VA v2; AI_basic (BI_relop t op)] [::$VA (VAL_int32 (wasm_bool (app_relop op v1 v2)))]
                     
   (** convert and reinterpret **)
   | rs_convert_success :
     forall t1 t2 v v' sx,
-    types_agree t1 v ->
+    types_agree (T_num t1) (VAL_num v) ->
     cvt t2 sx v = Some v' ->
-    reduce_simple [::AI_basic (BI_const v); AI_basic (BI_cvtop t2 CVO_convert t1 sx)] [::AI_basic (BI_const v')]
+    reduce_simple [::$VA v; AI_basic (BI_cvtop t2 CVO_convert t1 sx)] [::$VA v']
   | rs_convert_failure :
     forall t1 t2 v sx,
-    types_agree t1 v ->
+    types_agree (T_num t1) (VAL_num v) ->
     cvt t2 sx v = None ->
-    reduce_simple [::AI_basic (BI_const v); AI_basic (BI_cvtop t2 CVO_convert t1 sx)] [::AI_trap]
+    reduce_simple [::$VA v; AI_basic (BI_cvtop t2 CVO_convert t1 sx)] [::AI_trap]
   | rs_reinterpret :
     forall t1 t2 v,
-    types_agree t1 v ->
-    reduce_simple [::AI_basic (BI_const v); AI_basic (BI_cvtop t2 CVO_reinterpret t1 None)] [::AI_basic (BI_const (wasm_deserialise (bits v) t2))]
+    types_agree (T_num t1) (VAL_num v) ->
+    reduce_simple [::$VA v; AI_basic (BI_cvtop t2 CVO_reinterpret t1 None)] [::$VA (wasm_deserialise (bits v) t2)]
 
   (** control-flow operations **)
   | rs_unreachable :
@@ -71,37 +70,15 @@ Inductive reduce_simple : seq administrative_instruction -> seq administrative_i
     reduce_simple [::AI_basic BI_nop] [::]
   | rs_drop :
     forall v,
-    reduce_simple [::AI_basic (BI_const v); AI_basic BI_drop] [::]
+    reduce_simple [::$VA v; AI_basic BI_drop] [::]
   | rs_select_false :
-    forall n v1 v2,
+    forall n v1 v2 ot,
     n = Wasm_int.int_zero i32m ->
-    reduce_simple [::AI_basic (BI_const v1); AI_basic (BI_const v2); AI_basic (BI_const (VAL_int32 n)); AI_basic BI_select] [::AI_basic (BI_const v2)]
+    reduce_simple [::$VA v1; $VA v2; $VA (VAL_int32 n); AI_basic (BI_select ot)] [::$VA v2]
   | rs_select_true :
-    forall n v1 v2,
+    forall n v1 v2 ot,
     n <> Wasm_int.int_zero i32m ->
-    reduce_simple [::AI_basic (BI_const v1); AI_basic (BI_const v2); AI_basic (BI_const (VAL_int32 n)); AI_basic BI_select] [::AI_basic (BI_const v1)]
-  | rs_block :
-      forall vs es n m t1s t2s,
-        const_list vs ->
-        length vs = n ->
-        length t1s = n ->
-        length t2s = m ->
-        reduce_simple (vs ++ [::AI_basic (BI_block (Tf t1s t2s) es)]) [::AI_label m [::] (vs ++ to_e_list es)]
-  | rs_loop :
-      forall vs es n m t1s t2s,
-        const_list vs ->
-        length vs = n ->
-        length t1s = n ->
-        length t2s = m ->
-        reduce_simple (vs ++ [::AI_basic (BI_loop (Tf t1s t2s) es)]) [::AI_label n [::AI_basic (BI_loop (Tf t1s t2s) es)] (vs ++ to_e_list es)]
-  | rs_if_false :
-      forall n tf e1s e2s,
-        n = Wasm_int.int_zero i32m ->
-        reduce_simple ([::AI_basic (BI_const (VAL_int32 n)); AI_basic (BI_if tf e1s e2s)]) [::AI_basic (BI_block tf e2s)]
-  | rs_if_true :
-      forall n tf e1s e2s,
-        n <> Wasm_int.int_zero i32m ->
-        reduce_simple ([::AI_basic (BI_const (VAL_int32 n)); AI_basic (BI_if tf e1s e2s)]) [::AI_basic (BI_block tf e1s)]
+    reduce_simple [::$VA v1; $VA v2; $VA (VAL_int32 n); AI_basic (BI_select ot)] [::$VA v1]
   | rs_label_const :
       forall n es vs,
         const_list vs ->
@@ -110,28 +87,28 @@ Inductive reduce_simple : seq administrative_instruction -> seq administrative_i
       forall n es,
         reduce_simple [::AI_label n es [::AI_trap]] [::AI_trap]
   | rs_br :
-      forall n vs es i LI lh,
+      forall n vs es (i: labelidx) LI (lh: lholed i),
         const_list vs ->
         length vs = n ->
-        lfilled i lh (vs ++ [::AI_basic (BI_br i)]) LI ->
+        lfilled lh (vs ++ [::AI_basic (BI_br i)]) LI ->
         reduce_simple [::AI_label n es LI] (vs ++ es)
   | rs_br_if_false :
       forall n i,
         n = Wasm_int.int_zero i32m ->
-        reduce_simple [::AI_basic (BI_const (VAL_int32 n)); AI_basic (BI_br_if i)] [::]
+        reduce_simple [::$VA (VAL_int32 n); AI_basic (BI_br_if i)] [::]
   | rs_br_if_true :
       forall n i,
         n <> Wasm_int.int_zero i32m ->
-        reduce_simple [::AI_basic (BI_const (VAL_int32 n)); AI_basic (BI_br_if i)] [::AI_basic (BI_br i)]
-  | rs_br_table : (* ??? *)
+        reduce_simple [::$VA (VAL_int32 n); AI_basic (BI_br_if i)] [::AI_basic (BI_br i)]
+  | rs_br_table :
       forall iss c i j,
         length iss > Wasm_int.nat_of_uint i32m c ->
         List.nth_error iss (Wasm_int.nat_of_uint i32m c) = Some j ->
-        reduce_simple [::AI_basic (BI_const (VAL_int32 c)); AI_basic (BI_br_table iss i)] [::AI_basic (BI_br j)]
+        reduce_simple [::$VA (VAL_int32 c); AI_basic (BI_br_table iss i)] [::AI_basic (BI_br j)]
   | rs_br_table_length :
       forall iss c i,
         length iss <= (Wasm_int.nat_of_uint i32m c) ->
-        reduce_simple [::AI_basic (BI_const (VAL_int32 c)); AI_basic (BI_br_table iss i)] [::AI_basic (BI_br i)]
+        reduce_simple [::$VA (VAL_int32 c); AI_basic (BI_br_table iss i)] [::AI_basic (BI_br i)]
   | rs_local_const :
       forall es n f,
         const_list es ->
@@ -140,173 +117,23 @@ Inductive reduce_simple : seq administrative_instruction -> seq administrative_i
   | rs_local_trap :
       forall n f,
         reduce_simple [::AI_local n f [::AI_trap]] [::AI_trap]
-  | rs_return : (* ??? *)
-      forall n i vs es lh f,
+  | rs_return :
+      forall n (i: labelidx) vs es (lh: lholed i) f,
         const_list vs ->
         length vs = n ->
-        lfilled i lh (vs ++ [::AI_basic BI_return]) es ->
+        lfilled lh (vs ++ [::AI_basic BI_return]) es ->
         reduce_simple [::AI_local n f es] vs
   | rs_tee_local :
       forall i v,
         is_const v ->
-        reduce_simple [::v; AI_basic (BI_tee_local i)] [::v; v; AI_basic (BI_set_local i)]
+        reduce_simple [::v; AI_basic (BI_local_tee i)] [::v; v; AI_basic (BI_local_set i)]
   | rs_trap :
-      forall es lh,
+      forall es (lh: lholed 0),
         es <> [::AI_trap] ->
-        lfilled 0 lh [::AI_trap] es ->
+        lfilled lh [::AI_trap] es ->
         reduce_simple es [::AI_trap]
   .
 
-(*
-Inductive reduce : store_record -> list value -> list administrative_instruction -> instance -> store_record -> list value -> list administrative_instruction -> Prop :=
-| r_simple :
-    forall e e' s vs i,
-      reduce_simple e e' ->
-      reduce s vs e i s vs e'
-| r_call :
-    forall s vs i j f,
-      sfunc s i j = Some f ->
-      reduce s vs [::AI_basic (Call j)] i s vs [::Invoke f]
-| r_call_indirect_success :
-    forall s i j cl c vs tf,
-      stab s i (Wasm_int.nat_of_uint i32m c) = Some cl ->
-      stypes s i j = Some tf ->
-      cl_type cl = tf ->
-      reduce s vs [::AI_basic (BI_const (VAL_int32 c)); AI_basic (Call_indirect j)] i s vs [::Invoke cl]
-| r_call_indirect_failure1 :
-    forall s i j c cl vs,
-      stab s i (Wasm_int.nat_of_uint i32m c) = Some cl ->
-      stypes s i j <> Some (cl_type cl) ->
-      reduce s vs [::AI_basic (BI_const (VAL_int32 c)); AI_basic (Call_indirect j)] i s vs [::AI_trap]
-| r_call_indirect_failure2 :
-    forall s i j c vs,
-      stab s i (Wasm_int.nat_of_uint i32m c) = None ->
-      reduce s vs [::AI_basic (BI_const (VAL_int32 c)); AI_basic (Call_indirect j)] i s vs [::AI_trap]
-| r_invoke_native :
-    forall cl t1s t2s ts es ves vcs n m k zs vs s i j,
-      cl = Func_native j (Tf t1s t2s) ts es ->
-      ves = v_to_e_list vcs ->
-      length vcs = n ->
-      length ts = k ->
-      length t1s = n ->
-      length t2s = m ->
-      n_zeros ts = zs ->
-      reduce s vs (ves ++ [::Invoke cl]) i s vs [::Local m j (vcs ++ zs) [::AI_basic (Block (Tf [::] t2s) es)]]
-| r_invoke_host_success :
-    forall cl f t1s t2s ves vcs m n s s' vcs' vs i,
-      cl = Func_host (Tf t1s t2s) f ->
-      ves = v_to_e_list vcs ->
-      length vcs = n ->
-      length t1s = n ->
-      length t2s = m ->
-      host_apply s (Tf t1s t2s) f vcs (* FIXME: hs *) = Some (s', vcs') ->
-      reduce s vs (ves ++ [::Invoke cl]) i s' vs (v_to_e_list vcs')
-| r_invoke_host_failure :
-    forall cl t1s t2s f ves vcs n m s vs i,
-      cl = Func_host (Tf t1s t2s) f ->
-      ves = v_to_e_list vcs ->
-      length vcs = n ->
-      length t1s = n ->
-      length t2s = m ->
-      reduce s vs (ves ++ [::Invoke cl]) i s vs [::AI_trap]
-| r_get_local :
-    forall vi v vs i j s,
-      length vi = j ->
-      reduce s (vi ++ [::v] ++ vs) [::AI_basic (Get_local j)] i s (vi ++ [::v] ++ vs) [::AI_basic (BI_const v)]
-| r_set_local :
-    forall vs j v i s vd,
-      length vs > j ->
-      reduce s vs [::AI_basic (BI_const v); AI_basic (Set_local j)] i s (set_nth vd vs j v) [::]
-| r_get_global :
-    forall s vs j i v,
-      sglob_val s i j = Some v ->
-      reduce s vs [::AI_basic (Get_global j)] i s vs [::AI_basic (BI_const v)]
-| r_set_global :
-    forall s i j v s' vs,
-      supdate_glob s i j v = Some s' ->
-      reduce s vs [::AI_basic (BI_const v); AI_basic (Set_global j)] i s' vs [::]
-| r_load_success :
-    forall s i t bs vs k a off m j,
-      smem_ind s i = Some j ->
-      List.nth_error s.(s_mems) j = Some m ->
-      load m (Wasm_int.N_of_uint i32m k) off (t_length t) = Some bs ->
-      reduce s vs [::AI_basic (BI_const (VAL_int32 k)); AI_basic (Load t None a off)] i s vs [::AI_basic (BI_const (wasm_deserialise bs t))]
-| r_load_failure :
-    forall s i t vs k a off m j,
-      smem_ind s i = Some j ->
-      List.nth_error s.(s_mems) j = Some m ->
-      load m (Wasm_int.N_of_uint i32m k) off (t_length t) = None ->
-      reduce s vs [::AI_basic (BI_const (VAL_int32 k)); AI_basic (Load t None a off)] i s vs [::AI_trap]
-| r_load_packed_success :
-    forall s i t tp vs k a off m j bs sx,
-      smem_ind s i = Some j ->
-      List.nth_error s.(s_mems) j = Some m ->
-      load_packed sx m (Wasm_int.N_of_uint i32m k) off (tp_length tp) (t_length t) = Some bs ->
-      reduce s vs [::AI_basic (BI_const (VAL_int32 k)); AI_basic (Load t (Some (tp, sx)) a off)] i s vs [::AI_basic (BI_const (wasm_deserialise bs t))]
-| r_load_packed_failure :
-    forall s i t tp vs k a off m j sx,
-      smem_ind s i = Some j ->
-      List.nth_error s.(s_mems) j = Some m ->
-      load_packed sx m (Wasm_int.N_of_uint i32m k) off (tp_length tp) (t_length t) = None ->
-      reduce s vs [::AI_basic (BI_const (VAL_int32 k)); AI_basic (Load t (Some (tp, sx)) a off)] i s vs [::AI_trap]
-| r_store_success :
-    forall t v s i j vs mem' k a off m,
-      types_agree t v ->
-      smem_ind s i = Some j ->
-      List.nth_error s.(s_mems) j = Some m ->
-      store m (Wasm_int.N_of_uint i32m k) off (bits v) (t_length t) = Some mem' ->
-      reduce s vs [::AI_basic (BI_const (VAL_int32 k)); AI_basic (BI_const v); AI_basic (Store t None a off)] i (upd_s_mem s (update_list_at s.(s_mems) j mem')) vs [::]
-| r_store_failure :
-    forall t v s i j m k off a vs,
-      types_agree t v ->
-      smem_ind s i = Some j ->
-      List.nth_error s.(s_mems) j = Some m ->
-      store m (Wasm_int.N_of_uint i32m k) off (bits v) (t_length t) = None ->
-      reduce s vs [::AI_basic (BI_const (VAL_int32 k)); AI_basic (BI_const v); AI_basic (Store t None a off)] i s vs [::AI_trap]
-| r_store_packed_success :
-    forall t v s i j m k off a vs mem' tp,
-      types_agree t v ->
-      smem_ind s i = Some j ->
-      List.nth_error s.(s_mems) j = Some m ->
-      store_packed m (Wasm_int.N_of_uint i32m k) off (bits v) (tp_length tp) = Some mem' ->
-      reduce s vs [::AI_basic (BI_const (VAL_int32 k)); AI_basic (BI_const v); AI_basic (Store t (Some tp) a off)] i (upd_s_mem s (update_list_at s.(s_mems) j mem')) vs [::]
-| r_store_packed_failure :
-    forall t v s i j m k off a vs tp,
-      types_agree t v ->
-      smem_ind s i = Some j ->
-      List.nth_error s.(s_mems) j = Some m ->
-      store_packed m (Wasm_int.N_of_uint i32m k) off (bits v) (tp_length tp) = None ->
-      reduce s vs [::AI_basic (BI_const (VAL_int32 k)); AI_basic (BI_const v); AI_basic (Store t (Some tp) a off)] i s vs [::AI_trap]
-| r_current_memory :
-    forall i j m n s vs,
-      smem_ind s i = Some j ->
-      List.nth_error s.(s_mems) j = Some m ->
-      mem_size m = n ->
-      reduce s vs [::AI_basic (Current_memory)] i s vs [::AI_basic (BI_const (VAL_int32 (Wasm_int.int_of_Z i32m (Z.of_nat n))))]
-| r_grow_memory_success :
-    forall s i j m n mem' vs c,
-      smem_ind s i = Some j ->
-      List.nth_error s.(s_mems) j = Some m ->
-      mem_size m = n ->
-      mem_grow m (Wasm_int.N_of_uint i32m c) = Some mem' ->
-      reduce s vs [::AI_basic (BI_const (VAL_int32 c)); AI_basic Grow_memory] i (upd_s_mem s (update_list_at s.(s_mems) j mem')) vs [::AI_basic (BI_const (VAL_int32 (Wasm_int.int_of_Z i32m (Z.of_nat n))))]
-| r_grow_memory_failure :
-    forall i j m n s vs c,
-      smem_ind s i = Some j ->
-      List.nth_error s.(s_mems) j = Some m ->
-      mem_size m = n ->
-      reduce s vs [::AI_basic (BI_const (VAL_int32 c)); AI_basic Grow_memory] i s vs [::AI_basic (BI_const (VAL_int32 int32_minus_one))]
-| r_label :
-    forall s vs es les i s' vs' es' les' k lh,
-      reduce s vs es i s' vs' es' ->
-      lfilled k lh es les ->
-      lfilled k lh es' les' ->
-      reduce s vs les i s' vs' les'
-| r_local :
-    forall s vs es i s' vs' es' n v0s j,
-      reduce s vs es i s' vs' es' ->
-      reduce s v0s [::Local n i vs es] j s' v0s [::Local n i vs' es'].
-*)
 
 Inductive reduce : host_state -> store_record -> frame -> list administrative_instruction ->
                    host_state -> store_record -> frame -> list administrative_instruction -> Prop :=
@@ -314,34 +141,73 @@ Inductive reduce : host_state -> store_record -> frame -> list administrative_in
       forall e e' s f hs,
         reduce_simple e e' ->
         reduce hs s f e hs s f e'
-
+  | r_block :
+    forall hs s f vs es n m tb t1s t2s,
+      expand f.(f_inst) tb = Some (Tf t1s t2s) ->
+      const_list vs ->
+      length vs = n ->
+      length t1s = n ->
+      length t2s = m ->
+      reduce hs s f (vs ++ [::AI_basic (BI_block tb es)]) hs s f [::AI_label m [::] (vs ++ to_e_list es)]
+  | rs_loop :
+      forall hs s f vs es n m tb t1s t2s,
+      expand f.(f_inst) tb = Some (Tf t1s t2s) ->
+      const_list vs ->
+      length vs = n ->
+      length t1s = n ->
+      length t2s = m ->
+      reduce hs s f (vs ++ [::AI_basic (BI_loop tb es)]) hs s f [::AI_label n [::AI_basic (BI_loop tb es)] (vs ++ to_e_list es)]
+  | rs_if_false :
+    forall hs s f c vs es1 es2 n m tb t1s t2s,
+      expand f.(f_inst) tb = Some (Tf t1s t2s) ->
+      c = Wasm_int.int_zero i32m ->
+      const_list vs ->
+      length vs = m ->
+      length t1s = m ->
+      length t2s = n ->
+      reduce hs s f (vs ++ [::$VA (VAL_int32 c); AI_basic (BI_if tb es1 es2)]) hs s f [::AI_label n [::] (vs ++ to_e_list es2)]
+  | rs_if_true :
+    forall hs s f c vs es1 es2 n m tb t1s t2s,
+      expand f.(f_inst) tb = Some (Tf t1s t2s) ->
+      c <> Wasm_int.int_zero i32m ->
+      const_list vs ->
+      length vs = m ->
+      length t1s = m ->
+      length t2s = n ->
+      reduce hs s f (vs ++ [::$VA (VAL_int32 c); AI_basic (BI_if tb es1 es2)]) hs s f [::AI_label n [::] (vs ++ to_e_list es1)]
   (** calling operations **)
   | r_call :
-      forall s f i a hs,
+      forall s f (i: funcidx) a hs,
         List.nth_error f.(f_inst).(inst_funcs) i = Some a ->
         reduce hs s f [::AI_basic (BI_call i)] hs s f [::AI_invoke a]
   | r_call_indirect_success :
-      forall s f i a cl c hs,
-        (*        stab s f.(f_inst) (Wasm_int.nat_of_uint i32m c) = Some cl ->*)
-        stab_addr s f (Wasm_int.nat_of_uint i32m c) = Some a ->
+      forall s f x (y: typeidx) a cl i hs,
+        stab_elem s f.(f_inst) x (Wasm_int.nat_of_uint i32m i) = Some (VAL_ref_func a) ->
         List.nth_error s.(s_funcs) a = Some cl ->
-        stypes s f.(f_inst) i = Some (cl_type cl) ->
-        reduce hs s f [::AI_basic (BI_const (VAL_int32 c)); AI_basic (BI_call_indirect i)] hs s f [::AI_invoke a]
+        List.nth_error f.(f_inst).(inst_types) y = Some (cl_type cl) ->
+        reduce hs s f [::$VA (VAL_int32 i); AI_basic (BI_call_indirect x y)] hs s f [::AI_invoke a]
   | r_call_indirect_failure1 :
-      forall s f i a cl c hs,
-(*        stab s f.(f_inst) (Wasm_int.nat_of_uint i32m c) = Some cl ->*)
-        stab_addr s f (Wasm_int.nat_of_uint i32m c) = Some a ->
+      forall s f x (y: typeidx) a cl i hs,
+        stab_elem s f.(f_inst) x (Wasm_int.nat_of_uint i32m i) = Some (VAL_ref_func a) ->
         List.nth_error s.(s_funcs) a = Some cl ->
-        stypes s f.(f_inst) i <> Some (cl_type cl) ->
-        reduce hs s f [::AI_basic (BI_const (VAL_int32 c)); AI_basic (BI_call_indirect i)] hs s f [::AI_trap]
+        List.nth_error f.(f_inst).(inst_types) y <> Some (cl_type cl) ->
+        reduce hs s f [::$VA (VAL_int32 i); AI_basic (BI_call_indirect x y)] hs s f [::AI_trap]
   | r_call_indirect_failure2 :
-      forall s f i c hs,
-(*        stab s f.(f_inst) (Wasm_int.nat_of_uint i32m c) = None ->*)
-        stab_addr s f (Wasm_int.nat_of_uint i32m c) = None ->
-        reduce hs s f [::AI_basic (BI_const (VAL_int32 c)); AI_basic (BI_call_indirect i)] hs s f [::AI_trap]
+      forall s f x (y: typeidx) a i hs,
+        stab_elem s f.(f_inst) x (Wasm_int.nat_of_uint i32m i) = Some (VAL_ref_func a) ->
+        List.nth_error s.(s_funcs) a = None ->
+        reduce hs s f [::$VA (VAL_int32 i); AI_basic (BI_call_indirect x y)] hs s f [::AI_trap]
+  | r_call_indirect_failure3 :
+      forall s f x (y: typeidx) i hs,
+        stab_elem s f.(f_inst) x (Wasm_int.nat_of_uint i32m i) = None ->
+        reduce hs s f [::$VA (VAL_int32 i); AI_basic (BI_call_indirect x y)] hs s f [::AI_trap]
+  | r_call_indirect_failure4 :
+      forall s f x (y: typeidx) i hs t,
+        stab_elem s f.(f_inst) x (Wasm_int.nat_of_uint i32m i) = Some (VAL_ref_null t) ->
+        reduce hs s f [::$VA (VAL_int32 i); AI_basic (BI_call_indirect x y)] hs s f [::AI_trap]
   | r_invoke_native :
       forall a cl t1s t2s ts es ves vcs n m k zs s f f' i hs,
-        List.nth_error s.(s_funcs) a = Some cl ->
+        List.nth_error s.(s_funcs) (N.to_nat a) = Some cl ->
         cl = FC_func_native i (Tf t1s t2s) ts es ->
         ves = v_to_e_list vcs ->
         length vcs = n ->
@@ -351,10 +217,10 @@ Inductive reduce : host_state -> store_record -> frame -> list administrative_in
         n_zeros ts = zs ->
         f'.(f_inst) = i ->
         f'.(f_locs) = vcs ++ zs ->
-        reduce hs s f (ves ++ [::AI_invoke a]) hs s f [::AI_local m f' [::AI_basic (BI_block (Tf [::] t2s) es)]]
+        reduce hs s f (ves ++ [::AI_invoke a]) hs s f [::AI_local m f' [::AI_label m [::] (to_e_list es)]]
   | r_invoke_host_success :
       forall a cl h t1s t2s ves vcs m n s s' r f hs hs',
-        List.nth_error s.(s_funcs) a = Some cl ->
+        List.nth_error s.(s_funcs) (N.to_nat a) = Some cl ->
         cl = FC_func_host (Tf t1s t2s) h ->
         ves = v_to_e_list vcs ->
         length vcs = n ->
@@ -364,7 +230,7 @@ Inductive reduce : host_state -> store_record -> frame -> list administrative_in
         reduce hs s f (ves ++ [::AI_invoke a]) hs' s' f (result_to_stack r)
   | r_invoke_host_diverge :
       forall a cl t1s t2s h ves vcs n m s f hs hs',
-        List.nth_error s.(s_funcs) a = Some cl ->
+        List.nth_error s.(s_funcs) (N.to_nat a) = Some cl ->
         cl = FC_func_host (Tf t1s t2s) h ->
         ves = v_to_e_list vcs ->
         length vcs = n ->
@@ -374,104 +240,121 @@ Inductive reduce : host_state -> store_record -> frame -> list administrative_in
         reduce hs s f (ves ++ [::AI_invoke a]) hs' s f (ves ++ [::AI_invoke a])
 
   (** get, set, load, and store operations **)
-  | r_get_local :
+  | r_local_get :
       forall f v j s hs,
-        List.nth_error f.(f_locs) j = Some v ->
-        reduce hs s f [::AI_basic (BI_get_local j)] hs s f [::AI_basic (BI_const v)]
-  | r_set_local :
+        List.nth_error f.(f_locs) (N.to_nat j) = Some v ->
+        reduce hs s f [::AI_basic (BI_local_get j)] hs s f [::AI_basic (BI_const v)]
+  | r_local_set :
       forall f f' i v s vd hs,
         f'.(f_inst) = f.(f_inst) ->
-        i < length f.(f_locs) ->
-        f'.(f_locs) = set_nth vd f.(f_locs) i v ->
-        reduce hs s f [::AI_basic (BI_const v); AI_basic (BI_set_local i)] hs s f' [::]
-  | r_get_global :
+        N.to_nat i < length f.(f_locs) ->
+        f'.(f_locs) = set_nth vd f.(f_locs) (N.to_nat i) v ->
+        reduce hs s f [::AI_basic (BI_const v); AI_basic (BI_local_set i)] hs s f' [::]
+  | r_global_get :
       forall s f i v hs,
-        sglob_val s f.(f_inst) i = Some v ->
-        reduce hs s f [::AI_basic (BI_get_global i)] hs s f [::AI_basic (BI_const v)]
-  | r_set_global :
+        sglob_val s f.(f_inst) (N.to_nat i) = Some v ->
+        reduce hs s f [::AI_basic (BI_global_get i)] hs s f [::AI_basic (BI_const v)]
+  | r_global_set :
       forall s f i v s' hs,
-        supdate_glob s f.(f_inst) i v = Some s' ->
-        reduce hs s f [::AI_basic (BI_const v); AI_basic (BI_set_global i)] hs s' f [::]
+        supdate_glob s f.(f_inst) (N.to_nat i) v = Some s' ->
+        reduce hs s f [::AI_basic (BI_const v); AI_basic (BI_global_set i)] hs s' f [::]
+               
+  (** table **)
+  | r_table_get_success :
+    forall x i tabv s f hs,
+      stab_elem s f.(f_inst) x (Wasm_int.nat_of_uint i32m i) = Some tabv ->
+      reduce hs s f [::$VA (VAL_int32 i); AI_basic (BI_table_get x)] hs s f [::AI_basic (BI_const (VAL_ref tabv))]
+  | r_table_get_failure :
+    forall x i s f hs,
+      stab_elem s f.(f_inst) x (Wasm_int.nat_of_uint i32m i) = None ->
+      reduce hs s f [::$VA (VAL_int32 i); AI_basic (BI_table_get x)] hs s f [::AI_trap]
+  | r_table_set_success :
+    forall x i tabv s s' f hs,
+      stab_update s f.(f_inst) x (Wasm_int.nat_of_uint i32m i) tabv = Some s' ->
+      reduce hs s f [::$VA (VAL_int32 i); AI_basic (BI_const (VAL_ref tabv)); AI_basic (BI_table_set x)] hs s' f [::]
+  | r_table_set_failure :
+    forall x i tabv s s' f hs,
+      stab_update s f.(f_inst) x (Wasm_int.nat_of_uint i32m i) tabv = None ->
+      reduce hs s f [::$VA (VAL_int32 i); AI_basic (BI_const (VAL_ref tabv)); AI_basic (BI_table_set x)] hs s' f [::]
+             
+  (** memory **)
   | r_load_success :
     forall s i f t bs k a off m hs,
       smem_ind s f.(f_inst) = Some i ->
       List.nth_error s.(s_mems) i = Some m ->
-      load m (Wasm_int.N_of_uint i32m k) off (t_length t) = Some bs ->
-      reduce hs s f [::AI_basic (BI_const (VAL_int32 k)); AI_basic (BI_load t None a off)] hs s f [::AI_basic (BI_const (wasm_deserialise bs t))]
+      load m (Wasm_int.N_of_uint i32m k) off (tnum_length t) = Some bs ->
+      reduce hs s f [::$VA (VAL_int32 k); AI_basic (BI_load t None a off)] hs s f [::$VA (wasm_deserialise bs t)]
   | r_load_failure :
     forall s i f t k a off m hs,
       smem_ind s f.(f_inst) = Some i ->
       List.nth_error s.(s_mems) i = Some m ->
-      load m (Wasm_int.N_of_uint i32m k) off (t_length t) = None ->
-      reduce hs s f [::AI_basic (BI_const (VAL_int32 k)); AI_basic (BI_load t None a off)] hs s f [::AI_trap]
+      load m (Wasm_int.N_of_uint i32m k) off (tnum_length t) = None ->
+      reduce hs s f [::$VA (VAL_int32 k); AI_basic (BI_load t None a off)] hs s f [::AI_trap]
   | r_load_packed_success :
     forall s i f t tp k a off m bs sx hs,
       smem_ind s f.(f_inst) = Some i ->
       List.nth_error s.(s_mems) i = Some m ->
-      load_packed sx m (Wasm_int.N_of_uint i32m k) off (tp_length tp) (t_length t) = Some bs ->
-      reduce hs s f [::AI_basic (BI_const (VAL_int32 k)); AI_basic (BI_load t (Some (tp, sx)) a off)] hs s f [::AI_basic (BI_const (wasm_deserialise bs t))]
+      load_packed sx m (Wasm_int.N_of_uint i32m k) off (tp_length tp) (tnum_length t) = Some bs ->
+      reduce hs s f [::$VA (VAL_int32 k); AI_basic (BI_load t (Some (tp, sx)) a off)] hs s f [::$VA (wasm_deserialise bs t)]
   | r_load_packed_failure :
     forall s i f t tp k a off m sx hs,
       smem_ind s f.(f_inst) = Some i ->
       List.nth_error s.(s_mems) i = Some m ->
-      load_packed sx m (Wasm_int.N_of_uint i32m k) off (tp_length tp) (t_length t) = None ->
-      reduce hs s f [::AI_basic (BI_const (VAL_int32 k)); AI_basic (BI_load t (Some (tp, sx)) a off)] hs s f [::AI_trap]
+      load_packed sx m (Wasm_int.N_of_uint i32m k) off (tp_length tp) (tnum_length t) = None ->
+      reduce hs s f [::$VA (VAL_int32 k); AI_basic (BI_load t (Some (tp, sx)) a off)] hs s f [::AI_trap]
   | r_store_success :
     forall t v s i f mem' k a off m hs,
-      types_agree t v ->
+      typeof_num v = t ->
       smem_ind s f.(f_inst) = Some i ->
       List.nth_error s.(s_mems) i = Some m ->
-      store m (Wasm_int.N_of_uint i32m k) off (bits v) (t_length t) = Some mem' ->
-      reduce hs s f [::AI_basic (BI_const (VAL_int32 k)); AI_basic (BI_const v); AI_basic (BI_store t None a off)] hs (upd_s_mem s (update_list_at s.(s_mems) i mem')) f [::]
+      store m (Wasm_int.N_of_uint i32m k) off (bits v) (tnum_length t) = Some mem' ->
+      reduce hs s f [::$VA (VAL_int32 k); $VA v; AI_basic (BI_store t None a off)] hs (upd_s_mem s (set_nth mem' s.(s_mems) i mem')) f [::]
   | r_store_failure :
     forall t v s i f m k off a hs,
-      types_agree t v ->
+      typeof_num v = t ->
       smem_ind s f.(f_inst) = Some i ->
       List.nth_error s.(s_mems) i = Some m ->
-      store m (Wasm_int.N_of_uint i32m k) off (bits v) (t_length t) = None ->
-      reduce hs s f [::AI_basic (BI_const (VAL_int32 k)); AI_basic (BI_const v); AI_basic (BI_store t None a off)] hs s f [::AI_trap]
+      store m (Wasm_int.N_of_uint i32m k) off (bits v) (tnum_length t) = None ->
+      reduce hs s f [::$VA (VAL_int32 k); $VA v; AI_basic (BI_store t None a off)] hs s f [::AI_trap]
   | r_store_packed_success :
     forall t v s i f m k off a mem' tp hs,
-      types_agree t v ->
+      typeof_num v = t ->
       smem_ind s f.(f_inst) = Some i ->
       List.nth_error s.(s_mems) i = Some m ->
       store_packed m (Wasm_int.N_of_uint i32m k) off (bits v) (tp_length tp) = Some mem' ->
-      reduce hs s f [::AI_basic (BI_const (VAL_int32 k)); AI_basic (BI_const v); AI_basic (BI_store t (Some tp) a off)] hs (upd_s_mem s (update_list_at s.(s_mems) i mem')) f [::]
+      reduce hs s f [::$VA (VAL_int32 k); $VA v; AI_basic (BI_store t (Some tp) a off)] hs (upd_s_mem s (set_nth mem' s.(s_mems) i mem')) f [::]
   | r_store_packed_failure :
     forall t v s i f m k off a tp hs,
-      types_agree t v ->
+      typeof_num v = t ->
       smem_ind s f.(f_inst) = Some i ->
       List.nth_error s.(s_mems) i = Some m ->
       store_packed m (Wasm_int.N_of_uint i32m k) off (bits v) (tp_length tp) = None ->
-      reduce hs s f [::AI_basic (BI_const (VAL_int32 k)); AI_basic (BI_const v); AI_basic (BI_store t (Some tp) a off)] hs s f [::AI_trap]
-
-  (** memory **)
-  | r_current_memory :
+      reduce hs s f [::$VA (VAL_int32 k); $VA v; AI_basic (BI_store t (Some tp) a off)] hs s f [::AI_trap]
+  | r_memory_size :
       forall i f m n s hs,
         smem_ind s f.(f_inst) = Some i ->
         List.nth_error s.(s_mems) i = Some m ->
         mem_size m = n ->
-        reduce hs s f [::AI_basic (BI_current_memory)] hs s f [::AI_basic (BI_const (VAL_int32 (Wasm_int.int_of_Z i32m (Z.of_nat n))))]
-  | r_grow_memory_success :
+        reduce hs s f [::AI_basic (BI_memory_size)] hs s f [::$VA (VAL_int32 (Wasm_int.int_of_Z i32m (Z.of_nat n)))]
+  | r_memory_grow_success :
     forall s i f m n mem' c hs,
       smem_ind s f.(f_inst) = Some i ->
       List.nth_error s.(s_mems) i = Some m ->
       mem_size m = n ->
       mem_grow m (Wasm_int.N_of_uint i32m c) = Some mem' ->
-      reduce hs s f [::AI_basic (BI_const (VAL_int32 c)); AI_basic BI_grow_memory] hs (upd_s_mem s (update_list_at s.(s_mems) i mem')) f [::AI_basic (BI_const (VAL_int32 (Wasm_int.int_of_Z i32m (Z.of_nat n))))]
-  | r_grow_memory_failure :
+      reduce hs s f [::$VA (VAL_int32 c); AI_basic BI_memory_grow] hs (upd_s_mem s (set_nth mem' s.(s_mems) i mem')) f [::$VA (VAL_int32 (Wasm_int.int_of_Z i32m (Z.of_nat n)))]
+  | r_memory_grow_failure :
       forall i f m n s c hs,
         smem_ind s f.(f_inst) = Some i ->
         List.nth_error s.(s_mems) i = Some m ->
         mem_size m = n ->
-        reduce hs s f [::AI_basic (BI_const (VAL_int32 c)); AI_basic BI_grow_memory] hs s f [::AI_basic (BI_const (VAL_int32 int32_minus_one))]
-
+        reduce hs s f [::$VA (VAL_int32 c); AI_basic BI_memory_grow] hs s f [::$VA (VAL_int32 int32_minus_one)]
   (** label and local **)
   | r_label :
-      forall s f es les s' f' es' les' k lh hs hs',
+      forall k s f es les s' f' es' les' (lh: lholed k) hs hs',
         reduce hs s f es hs' s' f' es' ->
-        lfilled k lh es les ->
-        lfilled k lh es' les' ->
+        lfilled lh es les ->
+        lfilled lh es' les' ->
         reduce hs s f les hs' s' f' les'
   | r_local :
       forall s f es s' f' es' n f0 hs hs',
